Continue to develop the DTMP theory

Tealeaves/Theory/DecoratedTraversableFunctor.v
@@ -599,7 +599,6 @@ Section lifting_relations.
     (Hshape: shape t = shape u):
     shape (dec T t) = shape (dec T u).
   Proof.
-    Set Printing Implicit.
     unfold dec.
     unfold Decorate_Mapdt.
     unfold shape.
@@ -613,7 +612,32 @@ Section lifting_relations.
     (Hshape: shape t = shape u):
     map (cojoin (E ×)) (dec T (same_shape_zip A B t u Hshape)) =
       dec T (same_shape_zip (E * A) (E * B) (dec T t) (dec T u) _).
-  *)
+   *)
+
+
+  Definition lift_relation_ctx {A B:Type}
+    (R: E * A -> E * B -> Prop): T A -> T B -> Prop :=
+    precompose (dec T) ∘ mapdt (T := T) (G := subset) R.
+
+  Lemma relation_ctx_spec1:
+    forall (A B: Type) (R: E * A -> E * B -> Prop) (t: T A) (u: T B),
+      lift_relation_ctx R t u <->
+        (exists a : Vector (plength t) (E * B),
+            traverse (G := subset) R (mapdt_contents t) a /\
+              mapdt_make t a = dec T u).
+  Proof.
+    intros.
+    unfold lift_relation_ctx.
+    unfold compose at 1.
+    unfold precompose.
+    rewrite (mapdt_repr (E := E) (T := T)).
+    unfold_ops @Map_subset.
+    compose near (mapdt_contents t).
+    rewrite (traverse_commutative_idem
+               (T' := Vector (plength t)) (E * A) (E * B) R).
+    reflexivity.
+  Qed.
+
 
 
 End lifting_relations.
