Tealeaves/Examples/RecBag/Syntax.v
@@ -289,3 +289,8 @@ Section lfg.
   Qed.
 
 End lfg.
+
+
+Section mapci.
+
+End mapci.
