Tealeaves/Functors/Batch2.v
@@ -1,0 +1,72 @@
+From Tealeaves Require Import
+  Classes.Categorical.Applicative.
+
+Import Applicative.Notations.
+
+(** * The [Batch] idiom *)
+(******************************************************************************)
+Inductive Batch2 (A1 A2 B1 B2 C : Type) : Type :=
+| Done2 : C -> Batch2 A1 A2 B1 B2 C
+| StepA : Batch2 A1 A2 B1 B2 (A2 -> C) -> A1 -> Batch2 A1 A2 B1 B2 C
+| StepB : Batch2 A1 A2 B1 B2 (B2 -> C) -> B1 -> Batch2 A1 A2 B1 B2 C.
+
+#[global] Arguments Done2 {A1 A2 B1 B2 C}%type_scope _.
+#[global] Arguments StepA {A1 A2 B1 B2 C}%type_scope _ _.
+#[global] Arguments StepB {A1 A2 B1 B2 C}%type_scope _ _.
+
+(** ** Functor instance *)
+(******************************************************************************)
+
+(** *** Map operations *)
+(******************************************************************************)
+Fixpoint map_Batch2 {A1 A2 B1 B2: Type} {C1 C2: Type} (f : C1 -> C2)
+  (b : Batch2 A1 A2 B1 B2 C1): Batch2 A1 A2 B1 B2 C2 :=
+  match b with
+  | Done2 c => Done2 (f c)
+  | StepA mk a => StepA (map_Batch2 (compose f) mk) a
+  | StepB mk b => StepB (map_Batch2 (compose f) mk) b
+  end.
+
+#[export] Instance Map_Batch2 {A1 A2 B1 B2: Type}: Map (Batch2 A1 A2 B1 B2) :=
+  @map_Batch2 A1 A2 B1 B2.
+
+(** ** Applicative instance *)
+(******************************************************************************)
+
+(** *** Operations *)
+(******************************************************************************)
+#[export] Instance Pure_Batch2 {A1 A2 B1 B2}: Pure (@Batch2 A1 A2 B1 B2) :=
+  @Done2 A1 A2 B1 B2.
+
+#[program] Fixpoint mult_Batch {A1 A2 B1 B2} {C1 C2: Type}
+  (b1 : Batch2 A1 A2 B1 B2 C1)
+  (b2 : Batch2 A1 A2 B1 B2 C2):
+  Batch2 A1 A2 B1 B2 (C1 * C2) :=
+    match b2 with
+    | Done2 c2 => map (F := Batch2 A1 A2 B1 B2) (fun (c1 : C1) => (c1, c2)) b1
+    | StepA mk a =>
+        StepA
+          (map (F := Batch2 A1 A2 B1 B2) strength_arrow (mult_Batch b1 mk))
+          a
+    | StepB mk b =>
+        StepB
+          (map (F := Batch2 A1 A2 B1 B2) strength_arrow (mult_Batch b1 mk))
+          b
+    end.
+
+#[export] Instance Mult_Batch2 {A1 A2 B1 B2: Type}:
+  Mult (Batch2 A1 A2 B1 B2) :=
+  fun C1 C2 => uncurry (@mult_Batch A1 A2 B1 B2 C1 C2).
+
+(** ** The <<runBatch>> operation *)
+(******************************************************************************)
+Fixpoint runBatch2 {A1 A2 B1 B2: Type}
+  (F : Type -> Type) `{Map F} `{Mult F} `{Pure F}
+  (ϕB : B1 -> F B2)
+  (ϕA : A1 -> F A2)
+  {C : Type} (b : Batch2 A1 A2 B1 B2 C) : F C :=
+  match b with
+  | Done2 c => pure c
+  | StepA mk a => runBatch2 F ϕB ϕA (C := A2 -> C) mk <⋆> ϕA a
+  | StepB mk b => runBatch2 F ϕB ϕA (C := B2 -> C) mk <⋆> ϕB b
+  end.
